Cleanup inference

theories/Environment.v
@@ -1,7 +1,9 @@
 Require Import Blech.Spec.
 Require Import Blech.SpecNotations.
+Require Blech.OptionNotations.
 
 Require Import Coq.Unicode.Utf8.
+Require Coq.Bool.Bool.
 Require Coq.Lists.List.
 
 Require Import FunInd.
@@ -116,3 +118,184 @@ Proof using.
       constructor.
       all: auto.
 Qed.
+
+Definition eq_environment Γ Γ': {Γ = Γ'} + {Γ ≠ Γ'}.
+Proof.
+  decide equality.
+  destruct a as [v t], p as [v' t'].
+  destruct (eq_var v v'), (eq_type t t').
+  all: subst.
+  - left.
+    auto.
+  - right.
+    intro p.
+    inversion p.
+    contradiction.
+  - right.
+    intro p.
+    inversion p.
+    contradiction.
+  - right.
+    intro p.
+    inversion p.
+    contradiction.
+Defined.
+
+Module ProofTree.
+  Import OptionNotations.
+
+  Inductive mem: Set :=
+  | mem_eq x t Γ
+  | mem_ne x t Γ y t': mem → mem.
+
+  Definition varof p :=
+    match p with
+    | mem_eq x _ _ => x
+    | mem_ne x _ _ _ _ _ => x
+    end.
+
+  Definition typeof p :=
+    match p with
+    | mem_eq _ t _ => t
+    | mem_ne _ t _ _ _ _ => t
+    end.
+
+  Definition envof p :=
+    match p with
+    | mem_eq x t Γ => cons (x, t) Γ
+    | mem_ne _ _ Γ y t' _ => cons (y, t') Γ
+    end.
+
+  #[local]
+  Definition test {P Q} (p: {P} + {Q}): bool := if p then true else false.
+
+  Function check (p: mem): bool :=
+    match p with
+    | mem_eq x t Γ => true
+    | mem_ne x t Γ y t' p =>
+        negb (test (eq_var x y))
+        && test (eq_var x (varof p))
+        && test (eq_type t (typeof p))
+        && test (eq_environment Γ (envof p))
+        && check p
+    end %bool.
+
+  Definition asserts (p: mem): Prop := Spec.mem (varof p) (typeof p) (envof p).
+
+  Lemma check_sound (p: mem): Bool.Is_true (check p) → asserts p.
+  Proof.
+    unfold asserts.
+    induction p.
+    all: cbn.
+    all: intros q.
+    - constructor.
+    - destruct eq_var, eq_var, eq_type, eq_environment, (check p).
+      all: try contradiction.
+      subst.
+      constructor.
+      all: auto.
+  Qed.
+
+  Lemma check_complete {x t Γ}:
+    Spec.mem x t Γ →
+    ∃ p,
+      x = varof p
+      ∧ t = typeof p
+      ∧ Γ = envof p
+      ∧ Bool.Is_true (check p).
+  Proof.
+    intro q.
+    induction q.
+    all: cbn.
+    - exists (mem_eq x t Γ).
+      cbn.
+      all: repeat split; auto.
+    - destruct IHq as [p' [? [? []]]].
+      exists (mem_ne x t Γ y t' p').
+      cbn.
+      subst.
+      all: repeat split; auto.
+      destruct (check p').
+      2: contradiction.
+      destruct eq_var.
+      1: subst; contradiction.
+      destruct eq_var, eq_type, eq_environment.
+      all: cbv.
+      all: auto.
+  Qed.
+
+  Function infer x Γ: option mem :=
+    if Γ is cons (y, t') T
+    then
+      if eq_var x y
+      then
+        Some (mem_eq x t' T)
+      else
+        do p ← infer x T ;
+        Some (mem_ne (varof p) (typeof p) (envof p) y t' p)
+    else
+      None.
+
+  Lemma varof_infer {x Γ p}: infer x Γ = Some p → varof p = x.
+  Proof.
+    generalize dependent p.
+    functional induction (infer x Γ).
+    all: intros ? q.
+    all: inversion q.
+    all: auto.
+    - assert (IHo' := IHo _ e1).
+      cbn.
+      auto.
+  Qed.
+
+  Lemma envof_infer {x Γ p}: infer x Γ = Some p → envof p = Γ.
+  Proof.
+    generalize dependent p.
+    functional induction (infer x Γ).
+    all: intros ? q.
+    all: inversion q.
+    all: auto.
+    - assert (IHo' := IHo _ e1).
+      cbn.
+      subst.
+      auto.
+  Qed.
+
+  Lemma infer_sound {x Γ p}:
+    infer x Γ = Some p → Bool.Is_true (check p).
+  Proof.
+    generalize dependent p.
+    induction Γ.
+    1: discriminate.
+    cbn.
+    destruct a as [y t'].
+    intro.
+    destruct eq_var.
+    - subst.
+      intro q.
+      inversion q.
+      subst.
+      cbn.
+      auto.
+    - destruct (infer x Γ) eqn:q.
+      2: discriminate.
+      rewrite (varof_infer q).
+      intro q'.
+      inversion q'.
+      cbn.
+      rewrite (varof_infer q).
+      assert (IHΓ' := IHΓ _ eq_refl).
+      destruct (check m).
+      2: contradiction.
+      destruct eq_environment.
+      2: contradiction.
+      destruct eq_type.
+      2: contradiction.
+      cbn.
+      destruct eq_var.
+      1: subst;contradiction.
+      destruct eq_var.
+      2: contradiction.
+      auto.
+  Qed.
+End ProofTree.
